ironfleet/src/Dafny/Distributed/Impl/Lock/Node.i.dfy
@@ -2,12 +2,14 @@ include "../../Protocol/Lock/Node.i.dfy"
 include "Message.i.dfy"
 include "../Common/UdpClient.i.dfy"
 include "../../Common/Logic/Option.i.dfy"
+include "PacketParsing.i.dfy"
 
 module Impl_Node_i {
 import opened Protocol_Node_i
 import opened Message_i
 import opened Common__UdpClient_i
 import opened Logic__Option_i
+import opened PacketParsing_i 
 
 datatype CNode = CNode(held:bool, epoch:uint64, my_index:uint64, config:Config)
 
@@ -45,21 +47,26 @@ method NodeInitImpl(my_index:uint64, config:Config) returns (node:CNode)
     node := CNode(my_index == 0, if my_index == 0 then 1 else 0, my_index, config);
 }
 
-method NodeGrantImpl(s:CNode) returns (s':CNode, packet:CLockPacket, ghost ios:seq<LockIo>)
+method NodeGrantImpl(s:CNode) returns (s':CNode, packet:Option<CLockPacket>, ghost ios:seq<LockIo>)
     requires CNodeValid(s);
     ensures  NodeGrant(AbstractifyCNode(s), AbstractifyCNode(s'), ios);
+    ensures  s'.my_index == s.my_index && s'.config == s.config;
     ensures  |ios| == 0 || |ios| == 1;
-    ensures  |ios| == 1 ==> ios[0].LIoOpSend? && ios[0].s == AbstractifyCLockPacket(packet);
+    ensures  packet.Some? ==> |ios| == 1 && ios[0].LIoOpSend? 
+                           && ios[0].s == AbstractifyCLockPacket(packet.v);
+    ensures    OptionCLockPacketValid(packet) 
+            && (packet.Some? ==> packet.v.src == s.config[s.my_index]); 
     ensures  CNodeValid(s');
 {
     if s.held && s.epoch < 0xFFFF_FFFF_FFFF_FFFF {
         s' := s[held := false];
         var dst_index := (s.my_index + 1) % uint64(|s.config|);
-        packet := LPacket(s.config[dst_index], s.config[s.my_index], CTransfer(s.epoch + 1));
-        ios := [LIoOpSend(AbstractifyCLockPacket(packet))];
+        packet := Some(LPacket(s.config[dst_index], s.config[s.my_index], CTransfer(s.epoch + 1)));
+        ios := [LIoOpSend(AbstractifyCLockPacket(packet.v))];
     } else {
         s' := s;
         ios := [];
+        packet := None();
     }
 }
 
@@ -67,12 +74,15 @@ method NodeAcceptImpl(s:CNode, transfer_packet:CLockPacket)
     returns (s':CNode, locked_packet:Option<CLockPacket>, ghost ios:seq<LockIo>)
     requires CNodeValid(s);
     ensures  NodeAccept(AbstractifyCNode(s), AbstractifyCNode(s'), ios);
+    ensures  s'.my_index == s.my_index && s'.config == s.config;
     ensures  |ios| == 1 || |ios| == 2;
     ensures  locked_packet.None? ==> |ios| == 1 && ios[0].LIoOpReceive? 
                                   && ios[0].r == AbstractifyCLockPacket(transfer_packet);
     ensures  locked_packet.Some? ==> |ios| == 2 
                                   && ios == [LIoOpReceive(AbstractifyCLockPacket(transfer_packet)), 
                                              LIoOpSend(AbstractifyCLockPacket(locked_packet.v))];
+    ensures    OptionCLockPacketValid(locked_packet) 
+            && (locked_packet.Some? ==> locked_packet.v.src == s.config[s.my_index]); 
     ensures  CNodeValid(s');
 {
     ios := [LIoOpReceive(AbstractifyCLockPacket(transfer_packet))];
